theories/LevelTwo_eq.v
@@ -1,0 +1,398 @@
+From Prototype Require Import Prelude Sig.
+
+Module Make (S : Sig).
+Definition arg_ty := @arg_ty (base S.t).
+
+(*********************************************************************************)
+(** *** Terms and substitutions. *)
+(*********************************************************************************)
+
+(** Terms and substitutions are indexed by kinds. *)
+Inductive kind := 
+| (** Term. *)
+  K_t : kind
+| (** Constructor argument. *)
+  K_a : arg_ty -> kind
+| (** List of constructor arguments. *)
+  K_al : list arg_ty -> kind
+| (** Substitution. *)
+  K_s : kind.  
+Derive NoConfusion for kind.
+
+(** Terms and substitutions are indexed by a scope. *)
+Inductive scope :=
+| (** Scope of a term, argument, or argument list. *)
+  S1 : nat -> scope
+| (** Scope of a substitution. *)
+  S2 : nat -> nat -> scope.
+Derive NoConfusion for scope.
+
+(** A term/substitution metavariable is encoded as a unique identifier (a natural).
+    When denoting a term, we have access to an environment which maps metavariable identifiers
+    to actual (denoted) terms. *)
+Definition mvar (k : kind) (s : scope) := nat.
+
+(** Terms over an abstract signature. 
+    Terms are indexed by a kind and a scope. *)
+Inductive term : kind -> scope -> Type :=
+| (** Term variable. *)
+  T_var {n} : fin n -> term K_t (S1 n)
+| (** Non-variable term constructor, applied to a list of arguments. *)
+  T_ctor {n} : forall c, term (K_al (ctor_type S.t c)) (S1 n) -> term K_t (S1 n)
+| (** Empty argument list. *)
+  T_al_nil {n} : term (K_al []) (S1 n)
+| (** Non-empty argument list. *)
+  T_al_cons {n ty tys} : term (K_a ty) (S1 n) -> term (K_al tys) (S1 n) -> term (K_al (ty :: tys)) (S1 n)
+| (** Base argument (e.g. bool or string). *)
+  T_abase {n} : forall b, denote_base S.t b -> term (K_a (AT_base b)) (S1 n)
+| (** Term argument. *)
+  T_aterm {n} : term K_t (S1 n) -> term (K_a AT_term) (S1 n)
+| (** Binder argument. *)
+  T_abind {n ty} : term (K_a ty) (S1 (S n)) -> term (K_a (AT_bind ty)) (S1 n)
+| (** Substitution applied to a term/argument/argument-list. *)
+  T_subst {n m k} : term k (S1 n) -> term K_s (S2 n m) -> term k (S1 m)
+| (** Shift substitution. *)
+  T_sshift {n} : forall k, term K_s (S2 n (k + n))
+| (** Cons substitution. *)
+  T_scons {n m} : term K_t (S1 m) -> term K_s (S2 n m) -> term K_s (S2 (S n) m)
+| (** Composition of substitutions. *)
+  T_scomp {n m o} : term K_s (S2 n m) -> term K_s (S2 m o) -> term K_s (S2 n o)
+| (** Metavariable. *)
+  T_mvar {k s} : mvar k s -> term k s.
+Derive Signature NoConfusion for term.
+
+(** The identity substitution. *)
+Definition sid {n} : term K_s (S2 n n) := T_sshift 0.
+
+#[local] Notation "↑ k" := (T_sshift k) (at level 0).
+#[local] Notation "t .: s" := (T_scons t s) (at level 60, right associativity).
+#[local] Notation "s1 >> s2" := (T_scomp s1 s2) (at level 50, left associativity).
+#[local] Notation "t '[:' s ']'" := (T_subst t s) (at level 15, s at level 0, no associativity).
+
+(** Lift a substitution through a binder. *)
+Equations up_subst {n m} (s : term K_s (S2 n m)) : term K_s (S2 (S n) (S m)) :=
+up_subst s := T_var fin_zero .: s >> ↑1.
+
+(*********************************************************************************)
+(** *** Axiomatic equality. *)
+(*********************************************************************************)
+
+(** [t =σ t'] means that the terms/substitutions [t] and [t'] are equal 
+    modulo the equational theory of sigma calculus. *)
+Reserved Notation "t1 '=σ' t2" (at level 75, no associativity).
+Inductive axiom_eq : forall {k s}, term k s -> term k s -> Prop :=
+
+(** Equivalence. *)
+
+| aeq_refl {k s} (t : term k s) : t =σ t
+| aeq_sym {k s} (t1 t2 : term k s) : t1 =σ t2 -> t2 =σ t1
+| aeq_trans {k s} (t1 t2 t3 : term k s) : t1 =σ t2 -> t2 =σ t3 -> t1 =σ t3
+
+(** Congruence. *)
+
+| aeq_congr_ctor {n} c (args1 args2 : term _ (S1 n)) : 
+    args1 =σ args2 -> T_ctor c args1 =σ T_ctor c args2
+| aeq_congr_al_cons {n ty tys} (a1 a2 : term (K_a ty) (S1 n)) (args1 args2 : term (K_al tys) (S1 n)) : 
+    a1 =σ a2 -> args1 =σ args2 -> T_al_cons a1 args1 =σ T_al_cons a2 args2
+| aeq_congr_aterm {n} (t1 t2 : term K_t (S1 n)) : 
+    t1 =σ t2 -> T_aterm t1 =σ T_aterm t2
+| aeq_congr_abind {n ty} (a1 a2 : term (K_a ty) (S1 (S n))) : 
+    a1 =σ a2 -> T_abind a1 =σ T_abind a2
+| aeq_congr_subst {n m k} (t1 t2 : term k (S1 n)) (s1 s2 : term K_s (S2 n m)) : 
+    t1 =σ t2 -> s1 =σ s2 -> t1[: s1 ] =σ t2[: s2 ] 
+| aeq_congr_scons {n m} (t1 t2 : term K_t (S1 m)) (s1 s2 : term K_s (S2 n m)) : 
+    t1 =σ t2 -> s1 =σ s2 -> t1 .: s1 =σ t2 .: s2
+| aeq_congr_scomp {n m o} (s1 s2 : term K_s (S2 n m)) (r1 r2 : term K_s (S2 m o)) : 
+    s1 =σ s2 -> r1 =σ r2 -> s1 >> r1 =σ s2 >> r2
+
+(** Apply a substitution to a variable. *)
+
+| aeq_sshift_var {n} (i : fin n) k : 
+    (T_var i)[: ↑k ] =σ T_var (fin_weaken k i)
+| aeq_scons_zero {n m} (t : term K_t (S1 m)) (s : term K_s (S2 n m)) :
+    (T_var fin_zero)[: t .: s] =σ t
+| aeq_scons_succ {n m} (i : fin n) (t : term K_t (S1 m)) (s : term K_s (S2 n m)) :
+    (T_var (fin_succ i))[: t .: s] =σ (T_var i)[: s]
+
+(** Apply a substitution to a term. *)
+
+| aeq_subst_ctor {n m} c (args : term (K_al _) (S1 n)) (s : term K_s (S2 n m)) : 
+    (T_ctor c args)[: s ] =σ T_ctor c (args[: s ])
+| aeq_subst_al_nil {n m} (s : term K_s (S2 n m)) : 
+    T_al_nil[: s ] =σ T_al_nil
+| aeq_subst_al_cons {n m ty tys} (a : term (K_a ty) (S1 n)) (args : term (K_al tys) (S1 n)) (s : term K_s (S2 n m)) : 
+    (T_al_cons a args)[: s ] =σ T_al_cons (a[: s]) (args[: s ])
+| aeq_subst_abase {n m} b x (s : term K_s (S2 n m)) : 
+    (T_abase b x)[: s ] =σ T_abase b x
+| aeq_subst_aterm {n m} (t : term K_t (S1 n)) (s : term K_s (S2 n m)) : 
+    (T_aterm t)[: s ] =σ T_aterm (t[: s ])
+| aeq_subst_abind {n m ty} (a : term (K_a ty) (S1 (S n))) (s : term K_s (S2 n m)) : 
+    (T_abind a)[: s ] =σ T_abind (a[: up_subst s ])
+| aeq_subst_subst {n m o k} (t : term k (S1 n)) (s1 : term K_s (S2 n m)) (s2 : term K_s (S2 m o)) :
+    t[: s1 ][: s2 ] =σ t[: s1 >> s2 ]
+| aeq_subst_t_mvar {n k} (v : mvar k (S1 n)) :
+    (T_mvar v)[: sid ] =σ T_mvar v 
+
+(** Substitution laws. *)
+
+| aeq_sshift_succ {n} k : 
+    @T_sshift n (S k) =σ ↑k >> ↑1
+| aeq_sshift_scons {n} :
+  T_var (@fin_zero n) .: ↑1 =σ ↑0  
+| aeq_sid_l {n m} (s : term K_s (S2 n m)) : 
+    sid >> s =σ s 
+| aeq_sid_r {n m} (s : term K_s (S2 n m)) : 
+    s >> sid =σ s 
+| aeq_assoc {n m o p} (s1 : term K_s (S2 n m)) (s2 : term K_s (S2 m o)) (s3 : term K_s (S2 o p)) : 
+    s1 >> (s2 >> s3) =σ (s1 >> s2) >> s3
+| aeq_distrib {n m o} (t : term K_t (S1 m)) (s1 : term K_s (S2 n m)) (s2 : term K_s (S2 m o)) : 
+    (t .: s1) >> s2 =σ t[: s2 ] .: s1 >> s2
+
+where "t1 '=σ' t2" := (axiom_eq t1 t2).
+Hint Constructors axiom_eq : core.
+
+(*********************************************************************************)
+(** *** Setoid rewrite support. *)
+(*********************************************************************************)
+
+#[global] Instance axiom_eq_equiv k s : Equivalence (@axiom_eq k s).
+Proof. constructor ; eauto. Qed.
+
+#[global] Instance t_ctor_proper n c : Proper (axiom_eq ==> axiom_eq) (@T_ctor n c).
+Proof. intros ???. apply aeq_congr_ctor ; auto. Qed.
+
+#[global] Instance t_al_cons_proper n ty tys : Proper (axiom_eq ==> axiom_eq ==> axiom_eq) (@T_al_cons n ty tys).
+Proof. intros ??????. apply aeq_congr_al_cons ; auto. Qed.
+
+#[global] Instance t_aterm_proper n : Proper (axiom_eq ==> axiom_eq) (@T_aterm n).
+Proof. intros ???. apply aeq_congr_aterm ; auto. Qed.
+
+#[global] Instance t_abind_proper n ty : Proper (axiom_eq ==> axiom_eq) (@T_abind n ty).
+Proof. intros ???. apply aeq_congr_abind ; auto. Qed.
+
+#[global] Instance t_subst_proper n m k : Proper (axiom_eq ==> axiom_eq ==> axiom_eq) (@T_subst n m k).
+Proof. intros ??????. apply aeq_congr_subst ; auto. Qed.
+
+#[global] Instance t_scons_proper n m : Proper (axiom_eq ==> axiom_eq ==> axiom_eq) (@T_scons n m).
+Proof. intros ??????. apply aeq_congr_scons ; auto. Qed.
+
+#[global] Instance t_scomp_proper n m o : Proper (axiom_eq ==> axiom_eq ==> axiom_eq) (@T_scomp n m o).
+Proof. intros ??????. apply aeq_congr_scomp ; auto. Qed.
+
+(*********************************************************************************)
+(** *** Normal forms. *)
+(*********************************************************************************)
+
+(** A term is in normal form if and only if:
+    - metavariables always appear to the left of a substitution or composition.
+    - no other term appears to the left of a substitution or composition. *)
+Inductive nf : forall {k s}, term k s -> Prop :=
+(** Structural rules. *)
+| nf_tvar {n} (i : fin n) : 
+    nf (T_var i)
+| nf_tctor {n} c (args : term _ (S1 n)) : 
+    nf args -> nf (T_ctor c args) 
+| nf_al_nil {n} : 
+    nf (@T_al_nil n)
+| nf_al_cons {n ty tys} (a : term (K_a ty) (S1 n)) (args : term (K_al tys) (S1 n)) :
+    nf a -> nf args -> nf (T_al_cons a args)
+| nf_abase {n} b x :
+    nf (@T_abase n b x) 
+| nf_aterm {n} (t : term K_t (S1 n)) :
+    nf t -> nf (T_aterm t)
+| nf_abind {n ty} (a : term (K_a ty) (S1 (S n))) :
+    nf a -> nf (T_abind a)
+| nf_sshift {n k} : 
+    nf (@T_sshift n k)
+| nf_scons {n m} (t : term K_t (S1 m)) (s : term K_s (S2 n m)) : 
+    nf t -> nf s -> nf (t .: s)
+(** Substitution and composition rules. *)
+| nf_subst_t {n m k} (xt : mvar k (S1 n)) (s : term K_s (S2 n m)) : 
+    nf (T_mvar xt [: s ])
+| nf_subst_s {n m o k} (xs : mvar K_s (S2 (k + S n) m)) (s : term K_s (S2 m o)) :
+    nf s -> nf (T_var fin_zero [: ↑k >> T_mvar xs ][: s])
+| nf_scomp {n m o k} (v : mvar K_s (S2 (k + n) m)) (s : term K_s (S2 m o)) :
+    nf s -> nf (↑k >> T_mvar v >> s).
+Hint Constructors nf : core.
+
+(*********************************************************************************)
+(** *** Term/substitution simplification. *)
+(*********************************************************************************)
+
+(*
+
+apply_subst : fin n -> subst n m -> term K_t m
+apply_subst i (shift k) := T_var (i + k)
+apply_subst 0 (t .: s) := t
+apply_subst (S i) (t .: s) := apply_subst i s
+apply_subst i (s1 >> s2) := push_subst (apply_subst i s1) s2
+
+push_subst : term k n -> subst n m -> term k m
+push_subst (T_var i) s := apply_subst i s
+push_subst (T_ctor c args) s := T_ctor c (push_subst args s)
+push_subst T_al_nil s := T_al_nil
+push_subst (T_al_cons a args) s := T_al_cons (push_subst a s) (push_subst args s)
+push_subst (T_abase b x) := T_abase b x
+push_subst (T_aterm t) s := T_aterm (push_subst t s)
+push_subst (T_abind a) s := T_abind (push_subst a (up_subst s))
+push_subst (t[s]) s' := t[simpl_comp s s']
+
+simpl_comp : subst n m -> subst m o -> subst n o
+simpl_comp (shift 0) s := s
+simpl_comp (shift (S i)) s := push_shift (simpl_comp (shift i) s)
+simpl_comp (t .: s) s' := t[s'] .: (s >> s')
+simpl_comp (s1 >> s2) s3 := s1 >> simpl_comp s2 s3
+
+push_shift : subst (S n) m -> subst n m
+push_shift (shift i) := shift (S i)
+push_shift (t .: s) := s
+push_shift (s1 >> s2) := simpl_comp (push_shift s1) s2
+
+*)
+
+(** Head of a normal form substitution. *)
+Equations head {n m} (s : term K_s (S2 (S n) m)) : term K_t (S1 m) :=
+head (↑ k) := T_var (fin_weaken k fin_zero) ;
+head (t .: _) := t ;
+head (↑k >> T_mvar xs >> s) := T_var fin_zero [: ↑k >> T_mvar xs ] [: s ] ;
+head s := T_var fin_zero [: s ].
+
+Lemma head_sound {n m} (s : term K_s (S2 (S n) m)) :
+  head s =σ T_var fin_zero [: s ].
+Proof. funelim (head s) ; simp head in * ; auto. Qed.
+
+Lemma head_nf {n m} (s : term K_s (S2 (S n) m)) :
+  nf s -> nf (head s).
+Proof. intros H. dependent elimination H ; simp head ; auto. Qed.
+
+(** Tail of a normal form substitution. *)
+Equations tail {n m} (s : term K_s (S2 (S n) m)) : term K_s (S2 n m) :=
+tail (↑ k) := _ ;
+tail (_ .: s) := s ;
+tail (↑k >> T_mvar xs >> s) := _ >> T_mvar xs >> s ;
+tail s := ↑1 >> s.
+Next Obligation. rewrite PeanoNat.Nat.add_succ_r. exact (↑ (S k)). Defined.
+Next Obligation. rewrite PeanoNat.Nat.add_succ_r. exact (↑ (S k)). Defined.
+
+Lemma tail_sound {n m} (s : term K_s (S2 (S n) m)) :
+  tail s =σ ↑1 >> s.
+Proof. 
+funelim (tail s) ; simp tail in * ; auto.
+Admitted.
+
+Lemma tail_nf {n m} (s : term K_s (S2 (S n) m)) :
+  nf s -> nf (tail s).
+Proof. intros H. dependent elimination H ; simp tail ; auto. Admitted.
+
+(** Apply a normal form substitution to a variable. *)
+Equations apply_subst {n m} (i : fin n) (s : term K_s (S2 n m)) : term K_t (S1 m) :=
+apply_subst fin_zero s := head s ;
+apply_subst (fin_succ i) s := apply_subst i (tail s).
+
+Lemma apply_subst_sound {n m} (i : fin n) (s : term K_s (S2 n m)) :
+  apply_subst i s =σ T_var i [: s ].
+Proof. 
+funelim (apply_subst i s).
+- now rewrite head_sound.
+- rewrite H. rewrite tail_sound. rewrite <-aeq_subst_subst, aeq_sshift_var.
+  reflexivity.
+Qed.
+
+Lemma apply_subst_nf {n m} (i : fin n) (s : term K_s (S2 n m)) :
+  nf s -> nf (apply_subst i s).
+Proof. 
+intros H. funelim (apply_subst i s) ; simp apply_subst.
+- now apply head_nf.
+- apply H. now apply tail_nf.
+Qed.
+
+(** Apply a normal form substitution to a normal form term. *)
+Equations simpl_subst {k n m} (t : term k (S1 n)) (s : term K_s (S2 n m)) : term k (S1 m) :=
+simpl_subst (T_var i) s := apply_subst i s ;
+simpl_subst (T_ctor c args) s := T_ctor c (simpl_subst args s) ;
+simpl_subst T_al_nil _ := T_al_nil ;
+simpl_subst (T_al_cons a args) s := T_al_cons (simpl_subst a s) (simpl_subst args s) ;
+simpl_subst (T_abase b x) s := T_abase b x ;
+simpl_subst (T_aterm t) s := T_aterm (simpl_subst t s) ;
+simpl_subst (T_abind a) s := T_abind (simpl_subst a (T_var fin_zero .: simpl_comp s (↑1))) ;
+simpl_subst (T_subst t s1) s2 := T_subst t (simpl_comp s1 s2) ;
+simpl_subst (T_mvar xt) s := T_subst (T_mvar xt) s
+(** Compose normal form substitutions. *)
+with simpl_comp {n m o} (s1 : term K_s (S2 n m)) (s2 : term K_s (S2 m o)) : term K_s (S2 n o) :=
+simpl_comp (↑k) s := (↑k) >> s ;
+simpl_comp (t1 .: s1) s2 := simpl_subst t1 s2 .: simpl_comp s1 s2 ;
+simpl_comp (s1 >> s1') s2 := s1 >> (simpl_comp s1' s2) ;
+simpl_comp (T_mvar xs) s := (T_mvar xs) >> s.
+
+(*Fixpoint simpl_subst {k n m} (t : term k (S1 n)) (s : term K_s (S2 n m)) {struct t} : term k (S1 m)
+    with simpl_comp {n m o} (s1 : term K_s (S2 n m)) (s2 : term K_s (S2 m o)) {struct s1} : term K_s (S2 n o).
+(* simpl_subst. *)
+- dependent destruction t. 
+  + exact (T_subst (T_var f) s).
+  + exact (T_ctor c (simpl_subst _ _ _ t s)).
+  + exact (T_al_nil).
+  + exact (T_al_cons (simpl_subst _ _ _ t1 s) (simpl_subst _ _ _ t2 s)).
+  + exact (T_abase b d).
+  + exact (T_aterm (simpl_subst _ _ _ t s)).
+  + exact (T_abind (simpl_subst _ _ _ t (up_subst s))).
+  + exact (T_subst t1 (simpl_comp _ _ _ t2 s)).
+(* simpl_comp. *)
+- dependent destruction s1.
+  + exact (T_scomp (T_sshift k) s2).
+  + exact (T_scons (simpl_subst _ _ _ s1_1 s2) (simpl_comp _ _ _ s1_2 s2)).
+  + exact (T_scomp s1_1 (simpl_comp _ _ _ s1_2 s2)).
+Qed.  *)   
+
+
+Lemma simpl_subst_sound {k n m} (t : term k (S1 n)) (s : term K_s (S2 n m)) :
+  simpl_subst t s =σ T_subst t s.
+Proof. Admitted.
+
+Definition simpl {k s} (t : term k s) : term k s.
+dependent induction t.
+- exact (T_var f).
+- exact (T_ctor c IHt).
+- exact (T_al_nil).
+- exact (T_al_cons IHt1 IHt2).
+- exact (T_abase b d).
+- exact (T_aterm IHt).
+- exact (T_abind IHt).
+- exact (simpl_subst t1 t2).
+- exact (T_sshift k).
+- exact (T_scons IHt1 IHt2).
+- exact (T_scomp IHt1 IHt2).
+Defined.  
+
+Lemma up_subst_sid n : up_subst (@sid n) =σ sid.
+Proof. 
+cbv [up_subst sid]. simpl. setoid_rewrite <-(aeq_sshift_succ 0).
+setoid_rewrite aeq_sshift_scons. reflexivity.
+Qed.
+
+Lemma subst_sid k n (t : term k (S1 n)) : t[: sid] =σ t.
+Proof.
+dependent induction t generalizing n ; try (now auto).
+- unfold sid. rewrite (aeq_sshift_var f 0). reflexivity.
+- rewrite aeq_subst_ctor. rewrite IHt ; auto.
+- rewrite aeq_subst_al_cons. rewrite IHt1, IHt2 ; auto.
+- rewrite aeq_subst_aterm. rewrite IHt ; auto.
+- rewrite aeq_subst_abind. rewrite up_subst_sid. rewrite IHt ; auto.
+- setoid_rewrite aeq_subst_subst. rewrite aeq_sid_r. reflexivity.
+Qed. 
+
+(** Main property: [simpl] is sound. *)
+Lemma simpl_sound {k s} (t : term k s) : simpl t =σ t.
+Proof.
+dependent induction t ; simpl ; try auto.
+- now rewrite simpl_subst_sound.
+- rewrite IHt1, IHt2. reflexivity.
+- rewrite IHt1, IHt2. reflexivity. 
+Qed.
+
+(** This lemma is a simple consequence of the soundness of [simpl]. 
+    We could also prove it directly by induction, e.g. if we need it to prove 
+    the soundness of [simpl]. *)
+#[global] Instance simpl_proper k s : Proper (axiom_eq ==> axiom_eq) (@simpl k s).
+Proof. intros ???. rewrite simpl_sound, simpl_sound. assumption. Qed.
+
+End Make.
